lib/ImmutableTrie.dfy
@@ -1,0 +1,130 @@
+include "./sets.dfy"
+module ImmutableTrie {
+    import opened SetCustom
+
+    datatype Trie2 = Trie2(children: map<char, Trie2>, isWord: bool)
+
+    predicate ValidTrie(t: Trie2) 
+    {
+        t !in t.children.Values &&
+        (forall x :: x in t.children.Values ==> ValidTrie(x))
+    }
+
+    ghost function ChildrenSet2(parent: Trie2): set<Trie2> 
+        decreases parent
+    {
+        Union(set x | x in parent.children.Values :: ChildrenSet2(x)) + {parent}
+    }
+
+    ghost function ChildrenSet(parent: Trie2, children: set<Trie2>, res: set<Trie2>): set<Trie2> 
+        requires children <= parent.children.Values
+        // requires ValidTrie(parent)
+        decreases parent, children
+    {
+        if children == {} then res else
+            var x :| x in children;
+            ChildrenSet(parent, children - {x}, res + ChildrenSet(x, x.children.Values, {x}))
+    }
+
+    ghost function TrieSet(parent: Trie2): set<Trie2> 
+        // requires ValidTrie(parent)
+        decreases parent
+    {
+        ChildrenSet(parent, parent.children.Values, {parent})
+    }
+
+
+    function InsertWord(t: Trie2, word: string): Trie2
+        decreases |word|
+    {
+        if |word| == 0 && t.isWord then
+            t
+        else if |word| == 0 && !t.isWord then
+            Trie2(t.children, true)
+        else
+            if word[0] in t.children then
+                Trie2(t.children[word[0] := InsertWord(t.children[word[0]], word[1..])], t.isWord)
+            else
+                Trie2(t.children[word[0] := InsertWord(Trie2(map[], false), word[1..])], t.isWord)
+    }
+
+    predicate HasWord(t: Trie2, word: string)
+        decreases |word|
+    {
+        if |word| == 0 then
+            t.isWord
+        else
+            if word[0] in t.children then
+                HasWord(t.children[word[0]], word[1..])
+            else
+                false
+    }
+
+    function DeleteWord(t: Trie2, word: string): Trie2
+        decreases |word|
+    {
+        if |word| == 0 then
+            Trie2(t.children, false)
+        else
+            if word[0] in t.children then
+                var child := DeleteWord(t.children[word[0]], word[1..]);
+                // Trie2(t.children[word[0] := DeleteWord(t.children[word[0]], word[1..])], t.isWord)
+                Trie2(map key | key in t.children && (
+                    (key != word[0] ==> t.children[key].isWord || t.children[key].children.Keys != {}) &&
+                    (key == word[0] ==> child.isWord || child.children.Keys != {})
+                ):: if key != word[0] then t.children[key] else child, t.isWord)
+            else
+                t
+    }
+
+    lemma ThereIsAMinimum(s: set<char>)
+        requires s != {}
+        ensures exists x :: x in s && forall y :: y in s ==> x <= y
+    {
+        assert s != {};
+        var x :| x in s;
+        if s == {x} {
+        } else {
+            var s' := s - {x};
+            assert s == s' + {x};
+            ThereIsAMinimum(s');
+        }
+    }
+
+    function SetToSequence(s: set<char>): seq<char>
+        ensures var q := SetToSequence(s); forall i :: 0 <= i < |q| ==> q[i] in s
+        ensures |SetToSequence(s)| == |s|
+        ensures forall p :: p in s ==> p in SetToSequence(s)
+    {
+    if s == {} then [] else
+        ThereIsAMinimum(s);
+        var x :| x in s && forall y :: y in s ==> x <= y;
+        [x] + SetToSequence(s - {x})
+    }
+
+    method testTrie2() {
+        var t2 := Trie2(map[], false);
+        t2 := InsertWord(t2, "hello");
+        t2 := InsertWord(t2, "hello!");
+        t2 := InsertWord(t2, "boo");
+        assert HasWord(t2, "hello");
+        assert HasWord(t2, "boo");
+        t2 := DeleteWord(t2, "hello");
+        assert !HasWord(t2, "hello");
+        assert HasWord(t2, "boo");
+        assert HasWord(t2, "hello!");
+    }
+
+    // function TrieToRegex(t: Trie2): string
+    // {
+    //     if t.children.Keys == {} then
+    //         ""
+    //     else
+    //         var children := SetToSequence(t.children.Keys);
+    //         assert forall c :: c in children ==> c in t.children.Keys;
+    //         var pairs := Map((c: char) requires c in t.children.Keys => (c, TrieToRegex(t.children[c])), children);
+    //         var ss := Map((p: (char, string)) => [p.0] + if p.1 != "" && Contains(p.1, "|") then "("+p.1+")" else p.1, pairs);
+    //         var s := sumSeq(ss, "|");
+    //         s + if t.isWord then "|" else ""
+    // }
+}
