lib/sets.dfy
@@ -1,0 +1,108 @@
+
+module SetCustom {
+    export reveals *
+
+    ghost function Union<T>(s: set<set<T>>): set<T> 
+    {
+        if s == {} then 
+            assert forall x :: x in s ==> x <= {};
+            {} 
+        else
+            var x :| x in s;
+            x + Union(s - {x})
+    }
+
+
+    lemma UnionPlusSuperset<T>(s: set<set<T>>, x: set<T>, y: set<T>)
+        requires x <= y
+        requires x in s
+        requires forall y :: y in s ==> y != {}
+        ensures Union(s)+y == Union(s-{x} + {y})
+        decreases s
+    {
+        if s == {} {
+
+        }else{
+            UnionPlusOne(s-{x}, x);
+            calc{
+                Union(s-{x}+{x});
+                Union(s-{x}) + x;
+                {assert s-{x}+{x} == s;} 
+                Union(s);
+            }
+            UnionPlusOneIdempotent(s-{x}, y);
+
+        }
+    }
+
+    lemma UnionPlusOneIdempotent<T>(s: set<set<T>>, x: set<T>)
+        requires x != {}
+        requires forall y :: y in s ==> y != {}
+        ensures Union(s + {x}) == Union(s) + x
+        decreases s
+    {
+        if s == {} {
+        } else if x !in s {
+            UnionPlusOne(s, x);
+        }else{
+            assert s+{x} == s;
+            assert Union(s+{x}) == Union(s);
+            UnionHasAll(s);
+        }
+    }
+    lemma UnionPlusOne<T>(s: set<set<T>>, x: set<T>)
+        requires x != {}
+        requires forall y :: y in s ==> y != {}
+        requires x !in s
+        ensures Union(s + {x}) == Union(s) + x
+        decreases s
+    {
+        if s == {} {
+        } else {
+            assert s+{x} != {};
+            var z :| z in s + {x} && Union(s+{x}) == z + Union((s+{x})- {z} );
+            if z == x {
+
+            }else {
+                UnionPlusOne(s-{z}, x);
+                assert s -{z} + {x} == s+{x}-{z};
+                UnionPlusOne(s-{z}, z);
+                assert s -{z} + {z} == s ;
+                calc {
+                    Union(s+{x});
+                    z + Union(s+ {x}-{z});
+                    Union(s+ {x}-{z})+z;
+                    Union(s-{z})+x+z;
+                    Union(s-{z})+z+x;
+                }
+            }
+        }
+    }
+
+    lemma UnionContains<T>(s: set<set<T>>, x: T)
+        requires x in Union(s)
+        ensures exists y :: y in s && x in y
+    {
+    }
+    
+    lemma UnionHasAll<T>(s: set<set<T>>)
+        ensures forall x :: x in s ==> x <= Union(s)
+        ensures forall y :: y in s ==> forall x :: x in y ==> x in Union(s)
+    {
+        if s == {} {
+        } else {
+            var x :| x in s && Union(s) == x + Union(s - {x});
+            UnionHasAll(s - {x});
+            forall y | y in s
+                ensures y <= x + Union(s-{x}) 
+            {
+                if y == x {
+                    assert y <= x;
+                } else {
+                    assert y in s-{x};
+                }
+            }
+        }
+    }
+
+}
